verify/Rwv.lean
@@ -12,3 +12,4 @@ import Rwv.Eidos.Eval
 import Rwv.Eidos.Machine
 import Rwv.Sim
 import Rwv.Correspond
+import Rwv.Correspond2
